src/euf/Euf.v
@@ -180,7 +180,7 @@ Section certif.
       apply C.interp_true.
       destruct (Form.check_form_correct interp_form_hatom interp_form_hatom_bv _ ch_form);trivial.
     Qed.
-    Hint Resolve valid_C_true.
+    Hint Resolve valid_C_true : smtcoq_euf.
 
     Local Notation interp := (Atom.interp t_i t_func t_atom).
 
@@ -210,9 +210,9 @@ Section certif.
       C.interp rho (get_eq (Lit.blit l) f).
     Proof.
       intros l f Hf;unfold get_eq.
-      case_eq (t_form.[Lit.blit l]);trivial;intros.
-      case_eq (t_atom.[i]);trivial;intros.
-      destruct b;trivial.
+      case_eq (t_form.[Lit.blit l]);trivial with smtcoq_euf;intros.
+      case_eq (t_atom.[i]);trivial with smtcoq_euf;intros.
+      destruct b;trivial with smtcoq_euf.
       generalize wt_t_atom;unfold Atom.wt;unfold is_true;
        rewrite PArray.forallbi_spec;intros.
       assert (i < length t_atom).
@@ -279,48 +279,48 @@ Section certif.
        C.interp rho (check_trans_aux t1 t2 eqs res c).
     Proof.
       induction eqs;simpl;intros.
-      apply get_eq_interp;intros.
+      - apply get_eq_interp;intros.
       match goal with |- context [if ?b then _ else _] => case_eq b end;
-       intros;trivial.
+       intros;trivial with smtcoq_euf.
       simpl;rewrite Lit.interp_lit;unfold Var.interp.
-      destruct H1;[ | rewrite H1,orb_true_r;auto].
+      destruct H1;[ | rewrite H1,orb_true_r;auto with smtcoq_euf smtcoq_core].
       rewrite orb_true_iff, !andb_true_iff in H7;destruct H7 as
         [[H7 H8] | [H7 H8]].
       rewrite eqb_spec in H7. rewrite eqb_spec in H8. subst.
-      tunicity. subst t. rewrite H4, H1;auto.
+      tunicity. subst t. rewrite H4, H1;auto with smtcoq_euf smtcoq_core.
       rewrite eqb_spec in H7. rewrite eqb_spec in H8. subst.
-      tunicity. subst t;rewrite interp_binop_eqb_sym in H1;rewrite H4, H1;auto.
-      apply get_eq_interp;intros.
+      tunicity. subst t;rewrite interp_binop_eqb_sym in H1;rewrite H4, H1;auto with smtcoq_euf smtcoq_core.
+      - apply get_eq_interp;intros.
       destruct (Int63Properties.reflect_eqb t2 b);subst;tunicity; try subst t.
-      apply (IHeqs u);trivial.
+      + apply (IHeqs u);trivial.
       simpl;unfold is_true;rewrite orb_true_iff.
       rewrite Lit.interp_nlit;unfold Var.interp.
-      (* Attention ici on utilise la decidabilit'e de l'egalit'e sur u *)
+      (* Warning: here, we use decidability of equality over u *)
       case_eq (rho (Lit.blit a));[rewrite H4; intros | simpl;auto].
       destruct H1;[left | auto].
       apply interp_binop_eqb_trans with (4:= H1);trivial.
       rewrite interp_binop_eqb_sym;trivial.
-      destruct (Int63Properties.reflect_eqb t2 a0); subst;tunicity; try subst t.
-      apply (IHeqs u);trivial.
+      + destruct (Int63Properties.reflect_eqb t2 a0); subst;tunicity; try subst t.
+      * apply (IHeqs u);trivial.
       simpl;unfold is_true;rewrite orb_true_iff.
       rewrite Lit.interp_nlit;unfold Var.interp.
-      (* Attention ici on utilise la decidabilit'e de l'egalit'e sur u *)
+      (* Warning: here, we use decidability of equality over u *)
       case_eq (rho (Lit.blit a));[rewrite H4; intros | simpl;auto].
       destruct H1;[left | auto].
       apply interp_binop_eqb_trans with (4:= H1);trivial.
-      destruct (Int63Properties.reflect_eqb t1 b);subst;tunicity; try subst t.
-      apply (IHeqs u);trivial.
+      * destruct (Int63Properties.reflect_eqb t1 b);subst;tunicity; try subst t.
+      -- apply (IHeqs u);trivial.
       simpl;unfold is_true;rewrite orb_true_iff.
       rewrite Lit.interp_nlit;unfold Var.interp.
-      (* Attention ici on utilise la decidabilit'e de l'egalit'e sur u *)
+      (* Warning: here, we use decidability of equality over u *)
       case_eq (rho (Lit.blit a));[rewrite H4; intros | simpl;auto].
       destruct H1;[left | auto].
       apply interp_binop_eqb_trans with (5:= H1);trivial.
-      destruct (Int63Properties.reflect_eqb t1 a0);[subst;tunicity;try subst t|auto].
+      -- destruct (Int63Properties.reflect_eqb t1 a0);[subst;tunicity;try subst t|auto with smtcoq_euf smtcoq_core].
       apply (IHeqs u);trivial.
       simpl;unfold is_true;rewrite orb_true_iff.
       rewrite Lit.interp_nlit;unfold Var.interp.
-      (* Attention ici on utilise la decidabilit'e de l'egalit'e sur u *)
+      (* Warning: here, we use decidability of equality over u *)
       case_eq (rho (Lit.blit a));[rewrite H4; intros | simpl;auto].
       destruct H1;[left | auto].
       apply interp_binop_eqb_trans with (5:= H1);trivial.
@@ -332,9 +332,9 @@ Section certif.
        C.interp rho (check_trans res eqs).
     Proof.
       unfold check_trans;intros res [ | leq eqs].
-      apply get_eq_interp;intros.
+      - apply get_eq_interp;intros.
       destruct (Int63Properties.reflect_eqb a b).
-      unfold C.interp; simpl; rewrite orb_false_r.
+      + unfold C.interp; simpl; rewrite orb_false_r.
       unfold Lit.interp; simpl; rewrite Lit.is_pos_lit.
       unfold Var.interp; simpl; rewrite Lit.blit_lit.
       rewrite H1.
@@ -344,12 +344,12 @@ Section certif.
       unfold Atom.interp_hatom.
       rewrite HHb;simpl;rewrite Typ.cast_refl;simpl.
       apply Typ.i_eqb_refl.
-      auto.
-      apply get_eq_interp;intros.
+      + auto with smtcoq_euf.
+      - apply get_eq_interp;intros.
       apply check_trans_aux_correct with t;trivial.
       simpl;rewrite Lit.interp_nlit;unfold Var.interp. rewrite <- H1.
       (* Attention ici on utilise la decidabilit'e de l'egalit'e sur t *)
-      destruct (rho (Lit.blit leq));auto.
+      destruct (rho (Lit.blit leq));auto with smtcoq_core.
     Qed.
 
     Inductive Forall2 A B (P:A->B->Prop) : list A -> list B -> Prop :=
@@ -362,16 +362,16 @@ Section certif.
       (Forall2 _ _ (fun a b => interp_hatom a = interp_hatom b) l r -> C.interp rho c) ->
       C.interp rho (build_congr lp l r c).
     Proof.
-      induction lp;destruct l;destruct r;simpl;trivial;intros.
+      induction lp;destruct l;destruct r;simpl;trivial with smtcoq_euf smtcoq_core;intros.
       apply H;constructor.
       destruct a.
       apply get_eq_interp;intros.
       match goal with |- context [if ?x then _ else _] =>
-       case_eq x;intros;auto end.
+       case_eq x;intros;auto with smtcoq_euf smtcoq_core end.
       apply IHlp;simpl;intros.
       rewrite Lit.interp_nlit;unfold Var.interp.
-      case_eq (rho (Lit.blit i1));intros;simpl;[ | auto].
-      apply H;constructor;trivial.
+      case_eq (rho (Lit.blit i1));intros;simpl;[ | auto with smtcoq_euf smtcoq_core].
+      apply H;constructor;trivial with smtcoq_euf smtcoq_core.
       generalize (Atom.check_aux_interp_hatom _ t_func _ wf_t_atom a), (Atom.check_aux_interp_hatom _ t_func _ wf_t_atom b). rewrite Typ.eqb_spec in H3. rewrite Typ.eqb_spec in H4. unfold Atom.get_type in H3, H4. rewrite H3,H4. intros [va HHa] [vb HHb].
       revert H7;rewrite H2;unfold Atom.apply_binop; simpl.
       unfold Atom.interp_hatom.
@@ -381,11 +381,11 @@ Section certif.
       rewrite orb_true_iff, !andb_true_iff in H5;destruct H5 as
         [ [H5 H7] | [H5 H7]].
       rewrite eqb_spec in H5. rewrite eqb_spec in H7. subst.
-      rewrite HHa, HHb;trivial.
+      rewrite HHa, HHb;trivial with smtcoq_euf smtcoq_core.
       rewrite eqb_spec in H5. rewrite eqb_spec in H7. subst.
-      rewrite HHa, HHb;trivial.
-      destruct (Int63Properties.reflect_eqb i i0);[subst | auto].
-      apply IHlp;intros;apply H;constructor;auto.
+      rewrite HHa, HHb;trivial with smtcoq_euf smtcoq_core.
+      destruct (Int63Properties.reflect_eqb i i0);[subst | auto with smtcoq_euf smtcoq_core].
+      apply IHlp;intros;apply H;constructor;auto with smtcoq_euf smtcoq_core.
     Qed.
 
     Lemma valid_check_congr :
@@ -393,71 +393,71 @@ Section certif.
           C.interp rho (check_congr leq eqs).
     Proof.
       unfold check_congr;intros leq eqs;apply get_eq_interp;intros.
-      case_eq (t_atom .[ a]);intros;auto;
-      case_eq (t_atom .[ b]);intros;auto.
+      case_eq (t_atom .[ a]);intros;auto with smtcoq_euf smtcoq_core;
+      case_eq (t_atom .[ b]);intros;auto with smtcoq_euf smtcoq_core.
       (* uop *)
-      destruct (Atom.reflect_uop_eqb u u0);[subst | auto].
+      destruct (Atom.reflect_uop_eqb u u0);[subst | auto with smtcoq_euf smtcoq_core].
       apply build_congr_correct;intros.
       simpl;rewrite Lit.interp_lit, orb_false_r;unfold Var.interp.
       rewrite H1.
       generalize (Atom.check_aux_interp_hatom _ t_func _ wf_t_atom a), (Atom.check_aux_interp_hatom _ t_func _ wf_t_atom b). rewrite Typ.eqb_spec in H2. rewrite Typ.eqb_spec in H3. unfold Atom.get_type in H2, H3. rewrite H2,H3. intros [va HHa] [vb HHb].
       unfold Atom.apply_binop;unfold Atom.interp_hatom;simpl.
       rewrite HHb, HHa. simpl.
-      rewrite Atom.t_interp_wf in HHa; auto. rewrite H4 in HHa. simpl in HHa.
-      rewrite Atom.t_interp_wf in HHb; auto. rewrite H5 in HHb. simpl in HHb.
+      rewrite Atom.t_interp_wf in HHa; auto with smtcoq_euf smtcoq_core. rewrite H4 in HHa. simpl in HHa.
+      rewrite Atom.t_interp_wf in HHb; auto with smtcoq_euf smtcoq_core. rewrite H5 in HHb. simpl in HHb.
       rewrite Typ.cast_refl;simpl.
       assert (Atom.Bval t_i t va = Atom.Bval t_i t vb).
        inversion H6;subst.
        unfold Atom.interp_hatom in H10.
-       rewrite <- HHa; rewrite <- HHb, H10;trivial.
+       rewrite <- HHa; rewrite <- HHb, H10;trivial with smtcoq_euf smtcoq_core.
        inversion H7.
-       apply Eqdep_dec.inj_pair2_eq_dec in H9;trivial.
+       apply Eqdep_dec.inj_pair2_eq_dec in H9;trivial with smtcoq_euf smtcoq_core.
        rewrite H9.
        apply Typ.i_eqb_refl.
-      intros x y;destruct (Typ.reflect_eqb x y);auto.
+      intros x y;destruct (Typ.reflect_eqb x y);auto with smtcoq_euf smtcoq_core.
       (* bop *)
-      destruct (Atom.reflect_bop_eqb b0 b1);[subst | auto].
+      destruct (Atom.reflect_bop_eqb b0 b1);[subst | auto with smtcoq_euf smtcoq_core].
       apply build_congr_correct;intros.
       simpl;rewrite Lit.interp_lit, orb_false_r;unfold Var.interp.
       rewrite H1.
       generalize (Atom.check_aux_interp_hatom _ t_func _ wf_t_atom a), (Atom.check_aux_interp_hatom _ t_func _ wf_t_atom b). rewrite Typ.eqb_spec in H2. rewrite Typ.eqb_spec in H3. unfold Atom.get_type in H2, H3. rewrite H2,H3. intros [va HHa] [vb HHb].
       unfold Atom.apply_binop. unfold Atom.interp_hatom;simpl.
       rewrite HHb, HHa;simpl.
-      rewrite Atom.t_interp_wf in HHa; auto. rewrite H4 in HHa. simpl in HHa.
-      rewrite Atom.t_interp_wf in HHb; auto. rewrite H5 in HHb. simpl in HHb.
+      rewrite Atom.t_interp_wf in HHa; auto with smtcoq_euf smtcoq_core. rewrite H4 in HHa. simpl in HHa.
+      rewrite Atom.t_interp_wf in HHb; auto with smtcoq_euf smtcoq_core. rewrite H5 in HHb. simpl in HHb.
       rewrite Typ.cast_refl;simpl.
       assert (Atom.Bval t_i t va = Atom.Bval t_i t vb).
        inversion H6;clear H6;subst.
        inversion H12;clear H12;subst.
        unfold Atom.interp_hatom in H10, H8.
-       rewrite <- HHa. rewrite <- HHb, H10, H8;trivial.
+       rewrite <- HHa. rewrite <- HHb, H10, H8;trivial with smtcoq_euf smtcoq_core.
       inversion H7.
-      apply Eqdep_dec.inj_pair2_eq_dec in H9;trivial.
+      apply Eqdep_dec.inj_pair2_eq_dec in H9;trivial with smtcoq_euf smtcoq_core.
       rewrite H9.
       apply Typ.i_eqb_refl.
-      intros x y;destruct (Typ.reflect_eqb x y);auto.
+      intros x y;destruct (Typ.reflect_eqb x y);auto with smtcoq_euf smtcoq_core.
       (* op *)
-      destruct (Int63Properties.reflect_eqb i i0);[subst | auto].
+      destruct (Int63Properties.reflect_eqb i i0);[subst | auto with smtcoq_euf smtcoq_core].
       apply build_congr_correct;intros.
       simpl;rewrite Lit.interp_lit, orb_false_r;unfold Var.interp.
       rewrite H1.
       generalize (Atom.check_aux_interp_hatom _ t_func _ wf_t_atom a), (Atom.check_aux_interp_hatom _ t_func _ wf_t_atom b). rewrite Typ.eqb_spec in H2. rewrite Typ.eqb_spec in H3. unfold Atom.get_type in H2, H3. rewrite H2,H3. intros [va HHa] [vb HHb].
       unfold Atom.apply_binop;unfold Atom.interp_hatom;simpl.
       rewrite HHb, HHa;simpl.
-      rewrite Atom.t_interp_wf in HHa; auto. rewrite H4 in HHa. simpl in HHa.
-      rewrite Atom.t_interp_wf in HHb; auto. rewrite H5 in HHb. simpl in HHb.
+      rewrite Atom.t_interp_wf in HHa; auto with smtcoq_euf smtcoq_core. rewrite H4 in HHa. simpl in HHa.
+      rewrite Atom.t_interp_wf in HHb; auto with smtcoq_euf smtcoq_core. rewrite H5 in HHb. simpl in HHb.
       rewrite Typ.cast_refl;simpl.
       assert (Atom.Bval t_i t va = Atom.Bval t_i t vb).
         rewrite <- HHa;rewrite <- HHb;destruct (t_func.[i0]).
         apply f_equal;clear HHa HHb va vb H5 H4.
-        induction H6;simpl;trivial.
+        induction H6;simpl;trivial with smtcoq_euf smtcoq_core.
         unfold Atom.interp_hatom in H4.
-        rewrite IHForall2, H4;trivial.
+        rewrite IHForall2, H4;trivial with smtcoq_euf smtcoq_core.
       inversion H7.
-      apply Eqdep_dec.inj_pair2_eq_dec in H9;trivial.
+      apply Eqdep_dec.inj_pair2_eq_dec in H9;trivial with smtcoq_euf smtcoq_core.
       rewrite H9.
       apply Typ.i_eqb_refl.
-      intros x y;destruct (Typ.reflect_eqb x y);auto.
+      intros x y;destruct (Typ.reflect_eqb x y);auto with smtcoq_euf smtcoq_core.
     Qed.
 
     Lemma valid_check_congr_pred :
@@ -465,11 +465,11 @@ Section certif.
           C.interp rho (check_congr_pred lpa lpb eqs).
     Proof.
       unfold check_congr_pred;intros.
-      case_eq (t_form.[Lit.blit lpa]);auto.
-      case_eq (t_form.[Lit.blit lpb]);auto;intros.
-      case_eq (t_atom.[i0]);auto; case_eq (t_atom.[i]);auto;intros.
+      case_eq (t_form.[Lit.blit lpa]);auto with smtcoq_euf smtcoq_core.
+      case_eq (t_form.[Lit.blit lpb]);auto with smtcoq_euf smtcoq_core;intros.
+      case_eq (t_atom.[i0]);auto with smtcoq_euf smtcoq_core; case_eq (t_atom.[i]);auto with smtcoq_euf smtcoq_core;intros.
       (* uop *)
-      destruct (Atom.reflect_uop_eqb u0 u);[subst | auto].
+      destruct (Atom.reflect_uop_eqb u0 u);[subst | auto with smtcoq_euf smtcoq_core].
       apply build_congr_correct;simpl;intros.
       rewrite orb_false_r, Lit.interp_lit, Lit.interp_nlit;unfold Var.interp.
       replace (rho (Lit.blit lpb)) with (rho (Lit.blit lpa)).
@@ -485,12 +485,12 @@ Section certif.
         rewrite H2, def_t_atom;discriminate.
       apply H4 in H5;apply H4 in H6;clear H4.
       unfold Atom.interp_form_hatom, Atom.interp_hatom;simpl.
-      rewrite !Atom.t_interp_wf, H1, H2;simpl;trivial.
+      rewrite !Atom.t_interp_wf, H1, H2;simpl;trivial with smtcoq_euf smtcoq_core.
       apply f_equal;apply f_equal.
-      inversion H3;clear H3;subst;trivial.
+      inversion H3;clear H3;subst;trivial with smtcoq_euf smtcoq_core.
 
       (* bop *)
-      destruct (Atom.reflect_bop_eqb b0 b);[subst | auto].
+      destruct (Atom.reflect_bop_eqb b0 b);[subst | auto with smtcoq_euf smtcoq_core].
       apply build_congr_correct;simpl;intros.
       rewrite orb_false_r, Lit.interp_lit, Lit.interp_nlit;unfold Var.interp.
       replace (rho (Lit.blit lpb)) with (rho (Lit.blit lpa)).
@@ -506,13 +506,13 @@ Section certif.
         rewrite H2, def_t_atom;discriminate.
       apply H4 in H5;apply H4 in H6;clear H4.
       unfold Atom.interp_form_hatom, Atom.interp_hatom;simpl.
-      rewrite !Atom.t_interp_wf, H1, H2;simpl;trivial.
+      rewrite !Atom.t_interp_wf, H1, H2;simpl;trivial with smtcoq_euf smtcoq_core.
       inversion H3;clear H3;subst.
       inversion H11;clear H11;subst.
-      apply f_equal; apply f_equal2;trivial.
+      apply f_equal; apply f_equal2;trivial with smtcoq_euf smtcoq_core.
 
       (* op *)
-      destruct (Int63Properties.reflect_eqb i2 i1);[subst | auto].
+      destruct (Int63Properties.reflect_eqb i2 i1);[subst | auto with smtcoq_euf smtcoq_core].
       apply build_congr_correct;simpl;intros.
       rewrite orb_false_r, Lit.interp_lit, Lit.interp_nlit;unfold Var.interp.
       replace (rho (Lit.blit lpb)) with (rho (Lit.blit lpa)).
@@ -528,11 +528,11 @@ Section certif.
         rewrite H2, def_t_atom;discriminate.
       apply H4 in H5;apply H4 in H6;clear H4.
       unfold Atom.interp_form_hatom, Atom.interp_hatom;simpl.
-      rewrite !Atom.t_interp_wf, H1, H2;simpl;trivial.
+      rewrite !Atom.t_interp_wf, H1, H2;simpl;trivial with smtcoq_euf smtcoq_core.
       apply f_equal;destruct (t_func.[i1]);apply f_equal.
       clear H H0 H1 H2 H5 H6.
-      induction H3;simpl;trivial.
-      unfold Atom.interp_hatom in H;rewrite H, IHForall2;trivial.
+      induction H3;simpl;trivial with smtcoq_euf smtcoq_core.
+      unfold Atom.interp_hatom in H;rewrite H, IHForall2;trivial with smtcoq_euf smtcoq_core.
     Qed.
 
   End Proof.
